\documentclass[12pt]{article}
\usepackage{amsmath}
\usepackage{amssymb}

\numberwithin{equation}{subsubsection}

\title{Calculus Reference Sheet}
\author{Roy Magen}
\date{ }
\begin{document}

	\newcommand{\differ}{d}

	\newcommand{\derivative}[2][x]{\frac{\differ #2}{\differ #1}}
	\newcommand{\integral}[2][x]{\int #2\,\differ #1}
	\newcommand{\arccsc}[0]{\,\text{arccsc}\,}
	\newcommand{\arcsec}[0]{\,\text{arcsec}\,}
	\newcommand{\arccot}[0]{\,\text{arccot}\,}

	\begin{titlepage}
	\maketitle
	\end{titlepage}
	
	\tableofcontents
	\pagebreak

	\section{General}
		\subsection{Fundamental Theorem}
			\begin{gather}
				\integral{_a^b f(x)} = \integral[b]{f(b)} - \integral[a]{f(a)}
			\end{gather}
	\section{Differentiation}
		\subsection{Methods}
			\subsubsection{First Principles}
				\begin{gather}
					\derivative{f(x)} = \lim_{h \,\to\, 0} \frac{f(x + h) - f(x)}{h}
				\end{gather}
			\subsubsection{Linearity}
				\begin{gather}
					\derivative{af(x)} = a\derivative{f(x)} \\
					\derivative{f(x) + g(x)} = \derivative{f(x)} +
					\derivative{g(x)} \\
					\therefore \derivative{af(x) + bg(x)} = a\derivative{f(x)}
					+ b\derivative{g(x)}
				\end{gather}
			\subsubsection{Power Rule}
				\begin{gather}
					\text{where } n = 0 \\
					\derivative{x^n} = \derivative{1} \\
					= \lim_{h \,\to\, 0} \frac{(1 + h) - 1}{h} \\
					= \lim_{h \,\to\, 0} \frac{h}{h} \\
					= 1 \\ \nonumber
					\\
					\text{where } n \neq 0 \\
					\derivative{x^n} = \lim_{h \,\to\, 0} \frac{(x+h)^n - x^n}{h} \\
					= \lim_{h \,\to\, 0} \frac{\sum_{k=0}^n \binom{n}{k}
					x^{n-k}h^k - x^n}{h} \\
					= \lim_{h \,\to\, 0} \frac{\sum_{k=1}^n \binom{n}{k}
					x^{n-k}h^k}{h} \\
					= \lim_{h \,\to\, 0} \sum_{k=1}^n \binom{n}{k} x^{n-k}h^{k-1} \\
					= \lim_{h \,\to\, 0} \binom{n}{1} x^{n-1} + \sum_{k=2}^n
					x^{n-k}h^{k-1} \\
					= nx^{n-1} \\ \nonumber
					\\
					\boxed{
					\derivative{x^n} =
						\begin{cases}
							0 & \text{if } n = 0 \\
							nx^{n-1} & \text{if } n
							\neq 0
						\end{cases}
					}
				\end{gather}
			\subsubsection{Product Rule}
				\begin{gather}
					\derivative{f(x)g(x)} = g(x)\derivative{f(x)} +
					f(x)\derivative{g(x)}
				\end{gather}
			\subsubsection{Quotient Rule}
				\begin{gather}
					\derivative{\frac{f(x)}{g(x)}} =
					\frac{g(x)\derivative{f(x)} -
					f(x)\derivative{g(x)}}{g(x)^2}
				\end{gather}
			\subsubsection{Chain Rule}
				\begin{gather}
					\derivative{f(g(x))} =
					\derivative[g(x)]{f(g(x))}\derivative{g(x)}
				\end{gather}
		\subsection{Exonential and Logarithmic}
			\begin{gather}
				e = \lim_{n \,\to\, \infty} \left(1 +
				\frac{1}{n}\right)^n
			\end{gather}
			\subsubsection{Exponential}
				\begin{gather}
					\derivative{e^x} = e^x \\
					\derivative{a^x} = a^x\ln a
				\end{gather}
			\subsubsection{Logarithmic}
				\begin{gather}
					\derivative{\ln x} = \frac{1}{x} \qquad x > 0 \\
					\derivative{\log_ax} = \frac{1}{x\ln a}
				\end{gather}
		\subsection{Trigonometric}
			\begin{gather}
				\lim_{\theta \,\to\, 0} \frac{\sin \theta}{\theta} =
				1
			\end{gather}
			\subsubsection{Functions}
				\begin{gather}
					\derivative{\sin x} = \cos x \\
					\derivative{\cos x} = -\sin x \\
					\derivative{\tan x} = \sec^2 x
				\end{gather}
			\subsubsection{Reciprocal Functions}
				\begin{gather}
					\derivative{\csc x} = -\csc x \cot x \\
					\derivative{\sec x} = \sec x \tan x \\
					\derivative{\cot x} = -\csc^2 x
				\end{gather}
			\subsubsection{Inverse Functions}
				\begin{gather}
					\derivative{\arcsin x} = \frac{1}{\sqrt{1 -
					x^2}} \\
					\derivative{\arccos x} = \frac{-1}{\sqrt{1 -
					x^2}}  \\
					\derivative{\arctan x} = \frac{1}{x^2 + 1}
				\end{gather}
			\subsubsection{Inverse Reciprocal Functions}
				\begin{gather}
					\derivative{\arccsc x} = \frac{-1}{x^2\sqrt{1
					- \frac{1}{x^2}}} \\
					\derivative{\arcsec x} = \frac{1}{x^2\sqrt{1
					- \frac{1}{x^2}}} \\
					\derivative{\arccot x} = \frac{-1}{x^2 + 1}
				\end{gather}
	\section{Integration}
		\subsection{Methods}
			\subsubsection{Linearity}
				\begin{gather}
					\integral{af(x)} = a\integral{f(x)} \\
					\integral{f(x) + g(x)} = \integral{f(x)} +
					\integral{g(x)} \\
					\therefore \integral{af(x) + bg(x)} = a\integral{f(x)}
					+ b\integral{g(x)}
				\end{gather}
			\subsubsection{Power Rule}
				\begin{gather}
					\integral{x^n} =
						\begin{cases}
							\ln |x| + C & \text{if }
							n = -1 \\
							\frac{x^{n+1}}{n+1} + C
							& \text{if } n \neq -1
						\end{cases}
				\end{gather}
			\subsubsection{Integration by Substitution}
				\begin{gather}
					\integral{\derivative[g(x)]{f(g(x)}\derivative{g(x)}}
					= f(g(x)) \\
					\int
					\derivative[g{x}]{f(g(x))}\,dg(x) =
					f(g(x))
				\end{gather}
			\subsubsection{Integration by Parts}
				\begin{gather}
					\integral{f(x)\derivative{g(x)}} \\
					= \integral{\derivative{f(x)g(x)}} -
					\integral{\derivative{f(x)}g(x)} \\
					= f(x)g(x) - \integral{\derivative{f(x)}g(x)}
					\\
					\integral{f(x)g(x)} = f(x)\integral{g(x)}
					- \integral{\integral{g(x)}\,\derivative{f(x)}}
				\end{gather}
		\subsection{Exponential and Logarithmic}
			\subsubsection{Exponential}
				\begin{gather}
					\integral{e^x} = e^x + C \\
					\integral{a^x} = \frac{a^x}{\ln a} + C
				\end{gather}
			\subsubsection{Logarithmic}
				\begin{gather}
					\integral{\ln x} = x(\ln x - 1) + C \\
					\integral{\log_ax} = x(\log_ax - \ln a) +
					C \qquad a \neq 0
				\end{gather}
		\subsection{Trigonometric}
			\subsubsection{Functions}
				\begin{gather}
					\integral{\sin x} = -\cos x + C \\
					\integral{\cos x} = \sin x + C \\
					\integral{\tan x} = -\ln |\cos x| + C \\
					= \ln |\sec x| + C
				\end{gather}
			\subsubsection{Reciprocal Functions}
				\begin{gather}
					\integral{\csc x} =
					\integral{\sec x} =
					\integral{\cot x} =
				\end{gather}
			\subsubsection{Inverse Functions}
				\begin{gather}
					\integral{\arcsin x} =
					\integral{\arccos x} =
					\integral{\arctan x} =
				\end{gather}
			\subsubsection{Inverse Reciprocal Functions}
				\begin{gather}
					\integral{\arccsc x} =
					\integral{\arcsec x} =
					\integral{\arccot x} =
				\end{gather}

\end{document}
