% vim: tw=0

\documentclass{article}
\usepackage{amsmath, amssymb, amsthm, mathtools}
\numberwithin{equation}{subsubsection}

\title{Calculus Notes}
\author{Roy Magen}
\date{ }

\newtheorem{lrule}{Rule}
\newtheorem{app}{Application}
\newtheorem{defn}{Definition}
\newtheorem*{prem}{Premise}
\newtheorem{thm}{Theorem}
\newtheorem{cor}[thm]{Corollary}

%\newtheorem{prop}{Property}
%\newtheorem{lemma}{Lemma}
%\newtheorem{axiom}{Axiom}

\newcommand{\fromb}[3]{\overbrace{#3}^{#1~\ref{#2}}}
\newcommand{\from}[3]{\overset{#1~\ref{#2}}{#3}}
\newcommand{\byb}[3]{\underbrace{#3}_{#1~\ref{#2}}}
\newcommand{\by}[3]{\underset{#1~\ref{#2}}{#3}}

\begin{document}

\begin{titlepage}
    \maketitle
\end{titlepage}
\tableofcontents
\pagebreak

% each property should be labeled as one (perhaps make a property environment)
% (as in book)
% consider first writing on paper in order to have condensed list of content
\section{Prologue}
    \subsection{Basic Properties of Numbers}
    \newcommand{\nums}{\{\text{ numbers }\}}
    All variables are assumed to be numbers.
	%\subsubsection{Properties of Addition}
	    \begin{lrule}\label{addassoc} $ \forall (a,b,c) : \quad a + (b + c) = (a + b) + c $ \end{lrule}
	    \begin{lrule}\label{addcomm} $ \forall (a,b) : \quad a + b = b + a $ \end{lrule}
	    \begin{lrule}\label{addid} $ \forall a : \quad a + 0 = 0 + a = a $ \end{lrule}
	    \begin{lrule}\label{addinv} $ \forall a \;\exists (-a) : \quad a + (-a) = (-a) + a = 0 $ \end{lrule}
	    \begin{defn} $ a - b \overset{def}{=} a + (-b) $ \end{defn}

	    \begin{thm}
		$ \forall a : \quad a + x = a \iff x = 0 $
		\begin{proof}
		    \begin{align}
			a + x &= a \\
			(-a) + (a + x) &= (-a) + a \\
			(\fromb{Rule}{addassoc}{(-a) + a}) + x &= \from{Rule}{addinv}{0} \\
			\from{Rule}{addinv}{0} + x &= 0 \\
			\from{Rule}{addid}{x} &= 0
		    \end{align}
		\end{proof}
	    \end{thm}

	%\subsubsection{Properties of Multiplication}
	    \begin{lrule}\label{multassoc} $ \forall (a,b,c) : \quad a(bc) = (bc)a $ \end{lrule} 
	    \begin{lrule}\label{multcomm} $ \forall (a,b,c) : \quad ab = ba $ \end{lrule}
	    \begin{lrule}\label{multid} $ \forall a : \quad a \cdot 1 = 1 \cdot a = a $ \end{lrule}
	    \begin{prem} $ 1 \neq 0 $ \end{lrule}
	    \begin{lrule}\label{multinv} $ \forall a \neq 0 \;\exists a^{-1} : \quad aa^{-1} = a^{-1}a = 1 $ \end{lrule}

	    \begin{thm}\label{eqfactors}
		$ \forall a : \quad ab = ac \wedge a \neq 0 \iff b = c $
		\begin{proof}
		    \begin{align}
			ab &= ac \quad \wedge a \neq 0 \\
			a^{-1}(ab) &= a^{-1}(ac) \quad \wedge a \neq 0 \\
			(\fromb{Rule}{multassoc}{a^{-1}a})b &= (\fromb{Rule}{multassoc}{a^{-1}a})c \quad \wedge a \neq 0 \\
			\fromb{Rule}{multinv}{1} \cdot b &= \fromb{Rule}{multinv}{1} \cdot c \\
			\from{Rule}{multid}{b} &= \from{Rule}{multid}{c}
		    \end{align}
		\end{proof}
	    \end{thm}

	%\subsubsection{Combined Properties}
	    \begin{lrule}\label{distrib} $ \forall (a,b,c) : \quad a(b + c) = ab + ac $ \end{lrule}

	    \begin{thm}\label{multby0}
		$ \forall a : \quad 0a = 0 $
		\begin{proof}
		    \begin{align}
			0a + 0a &= 0a + 0a \\
			0a + 0a &= \from{Rule}{distrib}{a(0 + 0)} \\
			0a + 0a &= \from{Rule}{addid}{0a} \\
			0a &= 0
		    \end{align}
		\end{proof}
	    \end{thm}

	    \begin{thm}\label{prodof0}
		$ ab = 0 \iff (a = 0 \vee b = 0) $
		\begin{proof}
		    \begin{align}
			a = 0 \wedge b = 0 &\from{Theorem}{multby0}{\iff} ab = 0 \\ % consider reformatting
			ab &= 0 \quad \wedge a \neq 0 \\
			a^{-1}(ab) &= 0a^{-1} \quad \wedge a \neq 0 \\
			(\fromb{Rule}{multassoc}{a^{-1}a})b &= \from{Theorem}{multby0}{0} \quad \wedge a \neq 0 \\
			\fromb{Rule}{multinv}{1}b &= 0 \\
			\from{Rule}{multid}{b} &= 0
		    \end{align}
		\end{proof}
	    \end{thm}

	    \begin{thm}\label{subtreq}
		$ a - b = b - a \iff a = b $
		\begin{proof}
		    \begin{align}
			a - b &= b - a \\
			(a - b) + b &= (b - a) + b \\
			a - (\fromb{Rule}{addassoc}{(-b) + b}) &= \fromb{Rule}{addcomm}{b + (b - a)} \\
			a - \from{Rule}{addinv}{0} &= (\fromb{Rule}{addassoc}{b + b}) - a \\
			\from{Rule}{addid}{a} &= (b + b) - a \\
			a + a &= ((b + b) - a) + a \\
			\from{Rule}{distrib}{a(1 + 1)} &= \from{Rule}{distrib}{b(1 + 1)} + (\fromb{Rule}{addassoc}{(-a) + a}) \\
			a(1 + 1) &= b(1 + 1) + \from{Rule}{addinv}{0} \\
			a(1 + 1) = b(1 + 1) &\from{Theorem}{eqfactors}{\iff} a = b
		    \end{align}
		\end{proof}
	    \end{thm}

	    \begin{thm}\label{distrofneg}
		$ \forall (a,b) : \quad (-a)b = -(ab) $
		\begin{proof}
		    \begin{align}
			(-a)b + ab &= (-a)b + ab \\
			(-a)b + ab &= \from{Rule}{distrib}{((-a) + a)b} \\
			(-a)b + ab &= \fromb{Rule}{addinv}{0}b \\
			(-a)b + ab &= \from{Theorem}{multby0}{0} \\
			((-a)b + ab) + (-(ab)) &= 0 + (-(ab)) \\
			(-a)b + (\fromb{Rule}{addassoc}{ab +(-(ab))}) &= \from{Rule}{addid}{-(ab)} \\
			(-a)b + \from{Rule}{addinv}{0} &= -(ab) \\
			\from{Rule}{addid}{(-a)b} &= -(ab)
		    \end{align}
		\end{proof}
	    \end{thm}
	    
	    \begin{thm}\label{prodofnegs}
		$ \forall (a,b) : \quad (-a)(-b) = ab $
		\begin{proof}
		    \begin{align}
			(-a)(-b) + (-a)b &= (-a)(-b) + (-a)b \\
			(-a)(-b) + (\from{Theorem}{distrofneg}{-(ab)}) &= \from{Rule}{distrib}{-a((-b) + b)} \\
			(-a)(-b) - ab &= -a(\fromb{Rule}{addinv}{0}) \\
			(-a)(-b) - ab &= \from{Theorem}{multby0}{0} \\
			((-a)(-b) - ab) + ab &= 0 + ab \\
			(-a)(-b) + (\fromb{Rule}{addassoc}{(-(ab)) + ab}) &= \from{Rule}{addid}{ab} \\
			(-a)(-b) + \from{Rule}{addinv}{0} &= ab \\
			\from{Rule}{addid}{(-a)(-b)} &= ab
		    \end{align}
		\end{proof}
	    \end{thm}

\end{document}
